sfi/abstract_slow.v
@@ -1,0 +1,53 @@
+Require Import ssreflect ssrfun ssrbool eqtype ssrnat seq.
+
+Require Import common.common.
+Require Import sfi.classes sfi.abstract.
+
+Module AbsSlow.
+
+Section WithClasses.
+
+Set Implicit Arguments.
+
+Context (t   : machine_types)
+        {ops : machine_ops t}
+        {ap  : abstract_params t}
+        {sfi_syscalls : sfi_syscall_params t}.
+
+Definition state := option (@Abs.state t ap).
+
+Inductive step (othercalls : list (@Abs.syscall t ap)) (s s' : state) : Prop :=
+| step_go   : forall MM MM'
+                     (PREV : s  = Some MM)
+                     (NEXT : s' = Some MM')
+                     (STEP : Abs.step othercalls MM MM'),
+                step othercalls s s'
+| step_stop : forall MM
+                     (PREV : s  = Some MM)
+                     (NEXT : s' = None)
+                     (STOP : forall MM', ~ Abs.step othercalls MM MM'),
+                step othercalls s s'.
+
+Theorem slow_same : forall othercalls MM MM',
+  step othercalls (Some MM) (Some MM') <-> Abs.step othercalls MM MM'.
+Proof.
+  move=> oc MM MM'; split.
+  - by move=> [? ? [<-] [<-]|].
+  - by move=> ?; eapply step_go.
+Qed.
+
+Theorem slow_stops_late : forall othercalls MM,
+  step othercalls (Some MM) None <-> forall MM', ~ Abs.step othercalls MM MM'.
+Proof.
+  move=> oc MM; split.
+  - by move=> [|? [<-]].
+  - by move=> NO; apply: step_stop.
+Qed.
+
+Theorem slow_stopped : forall othercalls s',
+  ~ step othercalls None s'.
+Proof. by move=> oc s' []. Qed.
+
+End WithClasses.
+
+End AbsSlow.
