sfi/haskell_notation.v
@@ -1,0 +1,14 @@
+Require Import lib.utils.
+
+(* Monadic function composition *)
+Definition opt_compose {A B C}
+                       (f : B -> option C)
+                       (g : A -> option B)
+                       : A -> option C :=
+  bind f ∘ g.
+Infix "<=<" := opt_compose (at level 30).
+Arguments opt_compose {A B C} f g / x.
+
+Infix "$"   := (fun f x => f x) (at level 150, left associativity).
+Infix "<$>" := option_map       (at level 130, left associativity).
+Infix "=<<" := bind             (at level 130, left associativity).
