sfi/refinementSA.v
@@ -1,0 +1,118 @@
+Require Import List. Import ListNotations.
+
+Require Import ssreflect ssrfun ssrbool eqtype ssrnat seq.
+
+Require Import lib.utils lib.ordered lib.partial_maps common.common.
+Require Import symbolic.symbolic symbolic.rules.
+Require Import sfi.haskell_notation.
+Require Import sfi.classes sfi.list_utils sfi.set_utils sfi.isolate_sets.
+Require Import sfi.abstract sfi.abstract_slow sfi.symbolic.
+
+Import DoNotation.
+
+Section RefinementSA.
+
+Set Implicit Arguments.
+
+Import PartMaps.
+
+(* I want to use S and I as variables. *)
+Let S := Datatypes.S.
+Let I := Logic.I.
+(* ssreflect exposes `succn' as a synonym for `S' *)
+Local Notation II := Logic.I.
+
+Context
+  (t            : machine_types)
+  {ops          : machine_ops t}
+  {spec         : machine_ops_spec ops}
+  {ap           : abstract_params t}
+  {ap_spec      : params_spec ap}
+  {sfi_syscalls : sfi_syscall_params t}
+  {smemory      : Type}
+  {smem_class   : partial_map smemory (word t) (atom (word t) (@Sym.stag t))}
+  {sregisters   : Type}
+  {sreg_class   : partial_map sregisters (reg t) (atom (word t) (@Sym.stag t))}.
+
+Notation word    := (word t).
+Notation stag    := (@Sym.stag t).
+Notation sym_sfi := (@Sym.sym_sfi t ops smemory smem_class sregisters sreg_class).
+
+Notation astate  := (@Abs.state t ap).
+Notation astate' := (@AbsSlow.state t ap).
+Notation sstate  := (@Symbolic.state t sym_sfi).
+
+Notation astep  := (Abs.step []).
+Notation astep' := (AbsSlow.step []).
+Notation sstep  := Sym.step.
+
+Notation satom  := (atom word stag).
+Notation svalue := (@val word stag).
+Notation slabel := (@common.tag word stag).
+
+Definition refine_pc_b (apc : word) (spc : satom) :=
+  match spc with
+    | spc' @ (Sym.PC _ _) => apc == spc'
+    | _                   => false
+  end.
+
+Definition refine_mem_loc_b (ax : word) (sx : satom) : bool :=
+  match sx with
+    | sx' @ (Sym.DATA _ I W) => is_set I && is_set W && (ax == sx')
+    | _                      => false
+  end.
+
+Definition refine_reg_b (ar : word) (sr : satom) : bool :=
+  match sr with
+    | sr' @ Sym.REG => ar == sr'
+    | _             => false
+  end.
+
+Definition refine_memory : memory -> smemory -> Prop :=
+  pointwise refine_mem_loc_b.
+
+Definition refine_registers : registers -> sregisters -> Prop :=
+  pointwise refine_reg_b.
+
+Section With_EqType_refine_compartment_b.
+Import Sym.
+Definition refine_compartment_b (c : Abs.compartment t)
+                                (smem : smemory) : bool :=
+  is_some $
+    let: Abs.Compartment A J S := c in
+    do! sxs <- map_options (get smem) A;
+    do! sc  <- stag_compartment =<< the (map slabel sxs); (* modulo emptiness *)
+    do! guard? forallb (set_elem sc) <$>
+                 map_options (stag_incoming ∘ slabel <=< get smem) J;
+    do! guard? forallb (set_elem sc) <$>
+                 map_options (stag_writers  ∘ slabel <=< get smem) S;
+    Some tt.
+End With_EqType_refine_compartment_b.
+
+Definition refine_compartments (C : list (Abs.compartment t))
+                               (smem : smemory) : Prop :=
+  forallb (refine_compartment_b ^~ smem) C = true.
+
+Record refine_astate (ast : astate) (sst : sstate) : Prop := RefineState
+  { pc_refined          : refine_pc_b         (Abs.pc ast)   (Symbolic.pc sst)
+  ; regs_refined        : refine_registers    (Abs.regs ast) (Symbolic.regs sst)
+  ; mems_refined        : refine_memory       (Abs.mem  ast) (Symbolic.mem  sst)
+  ; compartments_refine : refine_compartments (Abs.compartments ast)
+                                              (Symbolic.mem sst)}.
+
+Inductive refine_astate' : astate' -> sstate -> Prop :=
+| refine_none : forall sst, (~ exists sst', sstep sst sst') ->
+                            refine_astate' None sst
+| refine_some : forall ast sst, refine_astate ast sst ->
+                                refine_astate' (Some ast) sst.
+
+Theorem backward_simulation : forall ast sst sst',
+  refine_astate' ast sst ->
+  sstep sst sst' ->
+  exists ast',
+    astep' ast ast' /\
+    refine_astate' ast' sst'.
+Proof.
+Abort.
+
+End RefinementSA.
